prove AtMostOneChosenImpliesAgreement

networkInvariantPrototypes/paxos/proof.dfy
@@ -122,10 +122,35 @@ module PaxosProof {
   *                                Application Invariants                                *
   ***************************************************************************************/
 
+  /*
+  1. Learn implies chosen.
+  2. chosen implies that is the only thing that can be chosen in all ballots.
+  */
+
+  // Util
+  // A quorum of Accept messages of the same vb
+  // Tony: Using monotonic transformations, I can push this to an acceptor host property,
+  // rather than a network property.
+  predicate Chosen(c: Constants, v: Variables, vb: ValBal) {
+    exists quorum: set<Message> :: 
+    && |quorum| >= c.f+1
+    && (forall m | m in quorum ::
+          && m.Accept?
+          && m in v.network.sentMsgs
+          && m.vb == vb
+    )
+  }
+
+  predicate AtMostOneChosenVal(c: Constants, v: Variables) {
+    forall vb1, vb2 | Chosen(c, v, vb1) && Chosen(c, v, vb2) 
+    :: vb1.v == vb2.v
+  }
+
+
   predicate ApplicationInv(c: Constants, v: Variables)
     requires v.WF(c)
   {
-    true
+    && AtMostOneChosenVal(c, v)
   }
 
   predicate Inv(c: Constants, v: Variables)
@@ -158,7 +183,73 @@ module PaxosProof {
     ensures Inv(c, v')
   {
     MessageInvInductive(c, v, v');
-    assume false;
+
+
+    assume AtMostOneChosenVal(c, v');
+    AtMostOneChosenImpliesAgreement(c, v');
+    assert Agreement(c, v');
+  }
+
+  // Lemma: For any Learn message, that learned value must have been chosen
+  lemma LearnedImpliesChosen(c: Constants, v: Variables, learnMsg: Message)
+    requires v.WF(c)
+    requires MessageInv(c, v)
+    requires learnMsg.Learn?
+    requires learnMsg in v.network.sentMsgs
+    ensures Chosen(c, v, VB(learnMsg.val, learnMsg.bal))
+  {
+    /* Suppose learnMsg(lnr, bal, val) in network. Then by LearnMsgsValid, lnr has a 
+      a quorum of receivedAccepts for vb := VB(bal, val). By LearnerValidReceivedAccepts,
+      there is a corresponding set of Accept(vb, _) messages in the network. */
+    var l := v.learners[learnMsg.lnr];
+    var vb := VB(learnMsg.val, learnMsg.bal);
+    var accQuorum := QuorumFromReceivedAccepts(l.receivedAccepts[vb], vb);  // witness
+  }
+
+
+  // Lemma: If at most one value can be chosen, then the Agreement property is true
+  lemma AtMostOneChosenImpliesAgreement(c: Constants, v: Variables) 
+    requires v.WF(c)
+    requires MessageInv(c, v)
+    requires AtMostOneChosenVal(c, v)
+    ensures Agreement(c, v)
+  {
+    /* Proof by contradiction. Suppose that v violates agreement, such that there are two
+      Learn messages with differnt values. Then by LearnedImpliesChosen, two different 
+      values are chosen, thus violating AtMostOneChosenVal */
+    if !Agreement(c, v) {
+      var m1, m2 :| 
+        && m1 in v.network.sentMsgs 
+        && m2 in v.network.sentMsgs 
+        && m1.Learn?
+        && m2.Learn?
+        && m1.val != m2.val;
+      LearnedImpliesChosen(c, v, m1);
+      LearnedImpliesChosen(c, v, m2);
+      assert false;
+    }
+  }
+
+  
+
+  /***************************************************************************************
+  *                                        Utils                                         *
+  ***************************************************************************************/
+  
+  lemma QuorumFromReceivedAccepts(s: set<AcceptorId>, vb: ValBal) returns (q: set<Message>)
+    decreases s
+    ensures |q| == |s|
+    ensures forall m | m in q :: m.Accept?
+    ensures forall m | m in q :: m.vb == vb
+    ensures forall m | m in q :: m.acc in s
+  {
+    if |s| == 0 {
+      return {};
+    } else {
+      var acc :| acc in s;
+      var subq := QuorumFromReceivedAccepts(s-{acc}, vb);
+      return subq + {Accept(vb, acc)};
+    }
   }
 }  // end module PaxosProof
 
